---
title: "Joint Probability for iid Variables"
format: gfm
editor: visual
---


## Problem

$$
\begin{align}
& \text{Prove that if} \quad X_1, X_2, \dots, X_n \overset{iid}{\sim} F(X), \quad \text{and}\\
& X_i ~~\text{is continuous variable}, \quad i \in (1, 2, \dots, n), \\
& \implies \mathcal{P}(X_{k_1} \leq X_{k_2} \leq X_{k_3} \leq \cdots \leq X_{k_n}) = \frac{1}{n!}, \\
& \text{and} \quad k_i \in (1, 2, 3, \dots, n), \quad k_i \ne k_j, ~~ \forall ~~ i, j \in  (1, 2, 3, \dots, n), ~~ i \ne j.
\end{align}
$$


\ 
\ 

## We will prove this relation for a specific case, we will generalize it for other cases.

\
\

$$
\begin{aligned}
& \text{if}\quad \langle k_1, k_2, k_3, \dots, k_n\rangle  = \langle 1, 2, 3, \dots, n \rangle \implies \\
& \mathbb{P} = \mathcal{P}(X_{k_1} \leq X_{k_2} \leq X_{k_3}\leq \cdots \leq X_{k_n}) = \mathcal{P}(X_1 \leq X_2 \leq X_3 \leq \cdots \leq X_n), \\
& \mathbb{P} = \int_{-\infty}^{+\infty}\int_{x_1}^{+\infty}\int_{x_2}^{+\infty}\int_{x_3}^{+\infty}\cdots\int_{x_{n-1}}^{+\infty}\prod_{i = 1}^n f(x_i)~dx_ndx_{n-1}dx_{n-2}\cdots dx_2dx_1 = \\
& \int_{-\infty}^{+\infty}f(x_1)\int_{x_1}^{+\infty}f(x_2)\int_{x_2}^{+\infty}f(x_3)\int_{x_3}^{+\infty}f(x_4)\cdots\int_{x_{n-1}}^{+\infty}f(x_n)dx_{n-1}dx_{n-2}\cdots dx_2dx_1 = \\
& \int_{-\infty}^{+\infty}f(x_1)\int_{x_1}^{+\infty}f(x_2)\int_{x_2}^{+\infty}f(x_3)\int_{x_3}^{+\infty}f(x_4)\cdots\int_{x_{n-1}}^{+\infty}\frac{d}{dx_n}F(x_n)dx_{n-1}dx_{n-2}\cdots dx_2dx_1, \\
\end{aligned}
$$



$$
\begin{aligned}
& \text{We know that if}~~X_i ~~\text{is continuous Variable}\implies F(X_i)\sim \text{Unif}(0, 1) \implies \\
& \mathbb{P} = \int_{-\infty}^{+\infty}f(x_1)\int_{x_1}^{+\infty}f(x_2)\cdots
\int_{x_{n-1}}^{+\infty}dF(x_{n})dx_{n-1}\cdots dx_2dx_1 = \\
& \int_{x_{n-1}}^{+\infty}f(x_1)\int_{x_2}^{+\infty}f(x_2)\cdots
\int_{x_{n-2}}^{+\infty}f(x_{n-1})(1 - F(x_{n-1}))dx_{n-1}\cdots dx_2dx_1 = \\
& \int_{x_{n-1}}^{+\infty}f(x_1)\int_{x_2}^{+\infty}f(x_2)\cdots
\int_{x_{n-2}}^{+\infty}\frac{d}{dx_{n-1}}F(x_{n-1})(1 - F(x_{n-1}))dx_{n-1}\cdots dx_2dx_1 = \\
& \int_{-\infty}^{+\infty}f(x_1) \int_{x_1}^{+\infty} f(x_2)\cdots \int_{F(x_{n-2})}^1 (1 - F(x_{n-1}))dF(x_{n-1})\cdots dx_1 =\\
& \int_{-\infty}^{+\infty}f(x_1)\int_{x_1}^{+\infty}\int\cdots\int_{x_{n-3}}^{+\infty}\frac{1}{2} - (F(x_{n-2}-\frac{F(x_{n-2})^2}{2}))dx_{n-2}\cdots dx_1, 
\end{aligned}
$$

##### as before


$$
\begin{aligned}
& \mathbb{P} = \int_{-\infty}^{+\infty}f(x_1)\int_{x_1}^{+\infty}\int\cdots\int_{x_{n-4}}^{+\infty}\frac{1}{3!} - (\frac{F(x_{n-3})}{2}-\frac{F(x_{n-3})^2}{2}+\frac{F(x_{n-3})^3}{3!})dF(x_{n-3})\cdots dx_1 = \\
& \int_{-\infty}^{+\infty}f(x_1)\int_{x_1}^{+\infty}\int\cdots\int_{x_{n-5}}^{+\infty}\frac{1}{4!} - (\frac{F(x_{n-4})}{3!}-\frac{F(x_{n-4})^2}{2\times 2!}+\frac{F(x_{n-3})^3}{3!} - \frac{F(x_{n-4})^4}{4!})dF(x_{n-4})\cdots dx_1, 
\end{aligned}
$$


##### If we continue in the same way, in the following, we will reach an expression set in the form below in each time of integration;


$$
\mathbb{P} = \int_{-\infty}^{+\infty} f(x_1) \int_{x_1}^{+\infty}f(x_2) \cdots \int_{x_{n-k}}^{+\infty}g(F(x_{n-(k-1)}), k)dF(x_{n-(k-1)})\cdots dx_1 \to 
$$